New proof for using relational properties

Vcg_Rela.v
@@ -234,15 +234,13 @@ Qed.
 
 (** Translation of a list of procedure call to Prop **)
 
-Parameter proc_call: Proc.Proc.t -> sigma -> sigma -> Prop.
+Definition proc_call f s s' ps := ceval (CCall f) s ps s'.
 
-Axiom test: forall y s s' ps, ceval (CCall y) s ps s' <-> proc_call y s s'.
-
-Program Fixpoint proc_to_pred p s s' (hy1:length p = length s) 
-                                     (hy2:length p = length s'): Prop:=
+Program Fixpoint proc_to_pred p s s' ps (hy1:length p = length s)
+                                        (hy2:length p = length s'): Prop:=
 match p, s, s' with
 | [] , [], [] => True
-| h :: q, s:: qs, s' :: qs' => proc_call h s s' /\ proc_to_pred q qs qs' _ _
+| h :: q, s:: qs, s' :: qs' => proc_call h s s' ps /\ proc_to_pred q qs qs' ps _ _
 | _, _, _ => !
 end.
 
@@ -320,15 +318,15 @@ destruct contra as (contra & _).
 discriminate contra.
 Defined.
 
-(** Facts about proc_to_pred**)
+(** Facts about proc_to_pred **)
 
 Lemma mk_proc_to_pred_def :
-forall c q s sl s' sl'
+forall c q s sl s' sl' ps
 (hy1:length (c::q) = length (s::sl)) (hy2:length (c::q) = length (s'::sl')),
 exists (hyr1:length q = length sl),
 exists (hyr2:length q = length sl'),
-proc_to_pred (c :: q) (s::sl) (s'::sl') hy1 hy2  =
-(proc_call c s s' /\ proc_to_pred q sl sl' hyr1 hyr2).
+proc_to_pred (c :: q) (s::sl) (s'::sl') ps hy1 hy2  =
+(proc_call c s s' ps /\ proc_to_pred q sl sl' ps hyr1 hyr2).
 Proof.
 intros.
 eexists.
@@ -337,7 +335,7 @@ program_simpl.
 Qed.
 
 Lemma rceval_proc_to_prod p s s' ps (hy1:length p = length s) (hy2:length p = length s') :
-proc_to_pred p s s' hy1 hy2 -> rceval (fold_call p) s ps s' .
+proc_to_pred p s s' ps hy1 hy2 -> rceval (fold_call p) s ps s' .
 Proof.
 generalize dependent hy2.
 generalize dependent hy1.
@@ -349,11 +347,11 @@ induction p; intros.
     simpl. apply E_Empty.
   + destruct s;[inversion hy1| ].
     destruct s';[inversion hy2| ].
-    specialize (mk_proc_to_pred_def a p s s0 s1 s' hy1 hy2) as (hyr1 & hyr2 & HYP).
+    specialize (mk_proc_to_pred_def a p s s0 s1 s' ps hy1 hy2) as (hyr1 & hyr2 & HYP).
     rewrite HYP in H.
     simpl.
     apply E_Seq.
-    - apply test. apply H.
+    -  apply H.
     - inversion hy1.
       inversion hy2.
      apply IHp with (hy1:= hyr1)(hy2:= hyr2). apply H.
@@ -361,10 +359,10 @@ Qed.
 
 (** Translation of a relational contract into Prop **)
 
-Definition tr (rcl:R_Phi.r_phi) :=
+Definition tr (rcl:R_Phi.r_phi) ps :=
    forall p s s' (hy1:length p = length s) (hy2:length p = length s'),
           0 < length p ->
-          proc_to_pred p s s' hy1 hy2 ->
+          proc_to_pred p s s' ps hy1 hy2 ->
           (get_r_pre (rcl p)) s -> (get_r_post (rcl p)) s' s.
 
 (** Facts about tr **)
@@ -372,7 +370,7 @@ Definition tr (rcl:R_Phi.r_phi) :=
 Lemma tr_relational_prop (rcl:R_Phi.r_phi) (ps: Psi.psi):
 (forall p, 0 < length p -> 
      relational_prop (get_r_pre (rcl p)) (get_r_post (rcl p)) (fold_call p) ps)
-          -> tr rcl.
+          -> tr rcl ps.
 Proof.
 intros H p s s' hy1 hy2 hy Hcall Hrp.
   apply H.
@@ -386,21 +384,23 @@ intros H p s s' hy1 hy2 hy Hcall Hrp.
     apply Hcall.
 Qed.
 
-(**  **)
+(** Adding proc_call to post condition of procedure contract **)
 
-Definition phi_call (cl : Phi.phi) := 
-    fun x => (get_pre (cl x), (fun m' m => (get_post (cl x)) m' m /\ proc_call x m m')).
+Definition phi_call (cl : Phi.phi) ps := 
+    fun x => (get_pre (cl x), (fun m' m => (get_post (cl x)) m' m /\ proc_call x m m' ps)).
+
+(** Facts about phi_call **)
 
 Lemma phi_call_hoare (ps: Psi.psi) (cl : Phi.phi) :
   (forall p, hoare_triple (get_pre (cl p)) (get_post (cl p)) (CCall p) ps) ->
-  (forall p, hoare_triple (get_pre (phi_call cl p)) (get_post (phi_call  cl p)) (CCall p) ps).
+  (forall p, hoare_triple (get_pre (phi_call cl ps p)) (get_post (phi_call cl ps p)) (CCall p) ps).
 Proof.
 intros.
 intros s s' Hpre Heval.
 split.
 * generalize p, s, s', Hpre, Heval.
   apply H.
-* eapply test. apply Heval.
+* apply Heval.
 Qed.
 
 (** Definition of a relational verification condition generator for procedures **)
@@ -440,10 +440,10 @@ rewrite hd_length_1 in Hpre by apply H2.
 assumption.
 Qed.
 
-Definition rtc_p (ps: Psi.psi) (cl : Phi.phi) (rcl : R_Phi.r_phi) : Prop :=
-    forall f m, 
+Definition rtc_p (ps: Psi.psi) (rcl : R_Phi.r_phi) : Prop :=
+    forall f m ps', 
     let c := (map ps f) in
     let h := (map (fun _ => []) f) in
     forall (hy1:length c = length m) (hy2:length c = length h),
-    (get_r_pre (rcl f)) m -> tr rcl -> rtc' c m h (phi_call (extract rcl)) hy1 hy2 /\
-                             rtc c m h (phi_call (extract rcl)) (fun m' _ => (get_r_post (rcl f)) m' m) hy1 hy2.
+    (get_r_pre (rcl f)) m -> tr rcl ps' -> rtc' c m h (phi_call (extract rcl) ps') hy1 hy2 /\
+                             rtc c m h (phi_call (extract rcl) ps') (fun m' _ => (get_r_post (rcl f)) m' m) hy1 hy2.
